Test/git-issues/git-issue-1604c.dfy
@@ -8,8 +8,18 @@ trait Tr { }
 class A extends Tr { }
 class B extends Tr { }
 
+predicate {:opaque} SpecialA(a: A) {
+  true
+}
+type Ap  = x : A | SpecialA(x)
+
 function method test(x: Tr): bool
   requires x is A
+{
+  if x is B then 1/0 == 0 else true
+}
+function method testSpecial(x: Tr): bool
+  requires x is A && SpecialA(x)
 {
   if x is B then 1/0 == 0 else true
 }
@@ -19,6 +29,8 @@ method Main() {
   var b := new B;
   var s: set<Tr> := {a, b};
   var aa := forall a': A :: a' in s ==> test(a');
+  var ap := forall a': Ap :: a' in s ==> test(a');
   assert(aa);
+  assert(ap);
   print "ok";
 }
